examples for the typed circuits, including a working teleport

Examples.v
@@ -1,132 +1,281 @@
+Require Import Program.
+Require Import Datatypes.
 Require Import Arith.
 Require Import List.
-Require Import Contexts.
+Require Import TypedCircuits.
+Import TC.
 Import ListNotations.
 Open Scope list_scope.
 
-(* Some wire patterns *)
-Definition q   := var 0.
-Definition w   := var 1.
-Definition w'  := var 2.
-Definition a   := var 3.
-Definition b   := var 4.
-Definition x   := var 5.
-Definition y   := var 6.
-Definition w1  := var 7.
-Definition w1' := var 8.
-Definition w2  := var 9.
-Definition w2' := var 10.
- 
-(* Getting contexts for input patterns *)
+(* Untyped patterns *)
+Inductive UPat := uvar : Var -> UPat | uunit | upair : UPat -> UPat -> UPat.
 
-Open Scope default_scope.
-
-Fixpoint get_singleton (v : Var) (W : WType) : Ctx := 
+(* Untyped to typed *)
+Fixpoint make_singleton (v : Var) (W : WType) : Ctx := 
   match v with
   | O => [Some W]
-  | (S v') => None :: get_singleton v' W
+  | (S v') => None :: make_singleton v' W
   end.
 
-Fixpoint manual_merge_atom (W1 W2 : option WType) : option WType := 
+Fixpoint make_SingletonCtx (v : Var) (W : WType) : 
+  SingletonCtx v W (make_singleton v W) :=
+  match v with
+  | O => SingletonHere W
+  | (S v') => SingletonLater _ _ _ (make_SingletonCtx v' W)
+  end.
+
+Fixpoint merge_atom (W1 W2 : option WType) : option WType := 
   match W1, W2 with
   | None, W' => W'
   | W', None => W'
   | _, _     => None (* ERROR CASE *) 
   end.
 
-Fixpoint manual_merge (ctx1 ctx2 : Ctx) : Ctx :=
-  match (ctx1, ctx2) with 
+Fixpoint merge (ctx1 ctx2 : Ctx) : Ctx :=
+  match ctx1, ctx2 with 
   | [], _ => ctx2
   | _, [] => ctx1
   | (c1 :: ctx1'), (c2 :: ctx2') => 
-    (manual_merge_atom c1 c2) :: (manual_merge ctx1' ctx2')
+    (merge_atom c1 c2) :: (merge ctx1' ctx2')
   end.
 
-Fixpoint make_context (p : Pat) (W : WType) : Ctx :=
+Fixpoint make_context (p : UPat) (W : WType) : Ctx :=
   match p with
-  | var v => get_singleton v W
-  | unit => []
-  | pair p1 p2 => match W with 
-               | W1 ⊗ W2 => manual_merge (make_context p1 W1) (make_context p2 W2)
+  | uvar v => make_singleton v W
+  | uunit => []
+  | upair p1 p2 => match W with 
+               | W1 ⊗ W2 => merge (make_context p1 W1) (make_context p2 W2)
                | _ => [] (* Fails *)
                end
   end.
 
+Lemma merge_eq : forall Γ1 Γ2 Γ3, MergeCtx Γ1 Γ2 Γ3 -> merge Γ1 Γ2 = Γ3.
+Proof.
+  intros.
+  generalize dependent Γ1. 
+  generalize dependent Γ2. 
+  induction Γ3.
+  + intros.
+    inversion H0; subst; reflexivity.
+  + intros.  
+    inversion H0; subst.
+    - reflexivity.
+    - reflexivity.
+    - simpl. 
+      rewrite IHΓ3; trivial.
+      inversion H5; reflexivity.
+Qed.
+
+(* Can turn into a function that returns an Option?
+Program Fixpoint type_pat (p : UPat) (W : WType) : (Pat (make_context p W) W) :=
+  match p with
+  | uvar v => var _ _ _ (make_SingletonCtx v W)
+  | uunit => unit 
+  | upair p1 p2 => match W with 
+                  | W1 ⊗ W2 => pair _ _ _ _ _ _ (type_pat p1 W1) (type_pat p2 W2)
+                  | _ => unit (* Really Fails *)
+                  end
+  end. 
+Next Obligation. 
+*)
+
+(* Alternatives for simple patterns *)
+
+(*
+Definition type_var (v : Var) (W : WType) : Pat (make_singleton v W) W :=
+  var _ _ _ (make_SingletonCtx v W).
+
+
+Search (_ <> _) bool.
+
+Program Definition type_pair (v1 v2 : Var) (W1 W2 : WType) {pf : (v1 =? v2) = false}: 
+  Pat (make_context (upair (uvar v1) (uvar v2)) (W1 ⊗ W2)) (W1 ⊗ W2) :=
+  pair _ _ _ _ _ _ (type_var v1 W1) (type_var v2 W2).
+Obligation 1. 
+  apply Nat.eqb_neq in pf. 
+  generalize dependent v2.
+  induction v1; intros.
+  destruct v2. tauto.
+  simpl; apply MergeCons; constructor.
+  simpl.
+  destruct v2.
+  simpl. apply MergeCons. constructor.
+  destruct (make_singleton v1 W1); simpl; constructor.
+  simpl.
+  constructor.
+  constructor.
+  apply IHv1.
+  intros Eq; subst; tauto.
+Defined.
+*)
+
+(* Projecting out elements of tensors *)
+Program Definition wproj {Γ W1 W2} (p : Pat Γ (Tensor W1 W2)) : 
+  {Γ1 : Ctx & Pat Γ1 W1 } * {Γ2 : Ctx & Pat Γ2 W2} :=
+  match p with 
+  | unit => _
+  | pair ctx1 ctx2 ctx w1 w2 M' p1 p2 => (existT _ ctx1 p1, existT _ ctx2 p2)  
+  end.
+
+(* Necessary associated lemma *)
+Lemma wproj_merge : forall Γ Γ1 Γ2 W1 W2 p1 p2 (p : Pat Γ (Tensor W1 W2)),
+  (existT (fun Γ1 : Ctx => Pat Γ1 W1) Γ1 p1, existT (fun Γ2 : Ctx => Pat Γ2 W2) Γ2 p2) 
+   = wproj p -> 
+  MergeCtx Γ1 Γ2 Γ.
+Proof.
+  intros Γ Γ1 Γ2 W1 W2 p1 p2 p H.
+  dependent destruction p.
+  inversion H0; subst.
+  assumption.
+Qed.
+
+(* Dangerous to take this notation *)
+Notation "a , b" := (Datatypes.pair a b) (at level 11, left associativity) : default_scope.
+(*
+Notation "w1 , w2" := (upair w1 w2) (at level 11, left associativity) : circ_scope.
+*)
+
+Notation "w1 , w2" := (pair _ _ _ _ _ _ w1 w2) (at level 11, left associativity) : circ_scope.
+
+Notation "(())" := unit : circ_scope.
+
+
+(* Some wire patterns *)
+Definition q : Var := 0.
+Definition w : Var  := 1.
+Definition w': Var  := 2.
+Definition a : Var  := 3.
+Definition b : Var  := 4.
+Definition x : Var  := 5.
+Definition y : Var  := 6.
+Definition w1 : Var := 7.
+Definition w1': Var := 8.
+Definition w2 : Var := 9.
+Definition w2': Var := 10.
+
+Check q.
+Check w1.
+ 
+(* Getting contexts for input patterns *)
+
+Open Scope circ_scope.
+
+(*** Tactics ***)
+
+Lemma merge_l_eq : forall Γ1 Γ2, MergeCtx [] Γ1 Γ2 -> Γ1 = Γ2.
+Proof. intros Γ1 Γ2 H. inversion H; subst; reflexivity. Qed.
+
+Lemma merge_r_eq : forall Γ1 Γ2, MergeCtx Γ1 [] Γ2 -> Γ1 = Γ2.
+Proof. intros Γ1 Γ2 H. inversion H; subst; reflexivity. Qed.
+
+Ltac find_pat := 
+  repeat match goal with 
+  | [ H : ?P |- ?P ] => exact H
+  | [ H : MergeCtx [] ?Γ1 ?Γ2 |- _] => apply merge_l_eq in H; subst
+  | [ H : MergeCtx ?Γ1 [] ?Γ2 |- _] => apply merge_r_eq in H; subst
+  end.
+
+Ltac type_check_circ := 
+  intros;
+  compute;
+  (* Compute in hyps will screw things up here *)
+  repeat match goal with 
+  | [ H : _  = wproj ?p |- _ ]      => apply wproj_merge in H
+  end;
+  compute in *;
+  repeat match goal with 
+  | [ |- ?Γ = ?Γ ]                  => reflexivity
+  (* from find_pat *)
+  | [ H : ?P |- ?P ]                => exact H
+  | [ H : MergeCtx [] ?Γ1 ?Γ2 |- _] => apply merge_l_eq in H; subst 
+  | [ H : MergeCtx ?Γ1 [] ?Γ2 |- _] => apply merge_r_eq in H; subst
+  | [ H : MergeCtx ?Γ1 ?Γ2 ?Γ3 |- MergeCtx ?Γ2 ?Γ1 ?Γ3 ] => apply (mergeSymm H)
+  | [ |- Pat [] One ]               => apply unit
+  | [ |- SingletonCtx _ ?W (?C :: [])]  => apply SingletonHere
+  | [ |- SingletonCtx _ ?W (None :: _)] => apply SingletonLater
+  (* From context checking *)
+  | [ |- MergeCtx [] _ _]           => apply MergeNilL
+  | [ |- MergeCtx _ [] _]           => apply MergeNilR
+  | [ |- MergeCtx _ _ []]           => apply MergeNilL (* Both work *)
+  end.
 
 (* Should be element of, but company coq is annoying *)
 (* Infix " ⊂ " := get_context (at level 50). *)
 
+(*
 Notation "'Box' w ⊂ W => C" := (box (make_context w W) w C _ _) (at level 60) 
                                : circ_scope.
+*)
 
-Close Scope default_scope.
-Open Scope circ_scope.
-
-
-(*** Tactics ***)
-
-Ltac type_check_circ :=
-  try (progress (
-  intros; compute; (* just to unfold obligations, actually *)
-  repeat (
-  [ > repeat match goal with
-  | [ |- Unitary _ ]              => constructor (* unique *)
-  | [ |- GateWType _ _ _ ]        => constructor (* unique *)
-  | [ |- SingletonCtx 0 _ _]      => apply SingletonHere (* unique *)
-  | [ |- SingletonCtx (S ?n) _ _] => apply SingletonLater (* unique *)
-  | [ |- EmptyCtx _ ]             => apply EmptyNil (* now only option *) 
-  | [ |- WF_Pat _ unit _ ]        => apply wf_unit (* unit case *)
-  | [ |- WF_Pat _ (var ?v) _ ]    => apply wf_var (* variable. w inferred later? *)
-  | [ |- WF_Pat _ (pair ?p1 ?p2) _ ]  => eapply wf_pair (* g1 g2 exist. quantified *)
-  end ..];
-  match goal with (* two ctxs must be concrete *)
-  | [ |- MergeCtx [] _ _]                        => apply MergeNilL
-  | [ |- MergeCtx _ [] _]                        => apply MergeNilR
-  | [ |- MergeCtx _ _ []]                        => apply MergeNilL (* Both work *)
-  | [ |- MergeCtx (?c1::?ctx1) (?c2::?ctx2) _]   => apply MergeCons
-  | [ |- MergeCtx (?c::?ctx) _ (?c::?ctx)]       => apply MergeNilR (* identical *)
-  | [ |- MergeCtx _ (?c::?ctx) (?c::?ctx)]       => apply MergeNilL (* identical *)
-  | [ |- MergeCtx (?c1::?ctx1) _  (?c::?ctx)]    => apply MergeCons (* distinct *)
-  | [ |- MergeCtx _ (?c2::?ctx2) (?c::?ctx)]     => apply MergeCons (* distinct *)
-  | [ |- MergeOption (Some ?w) _ _]              => apply MergeLeft
-  | [ |- MergeOption _ (Some ?w) _]              => apply MergeRight
-  | [ |- MergeOption None None _]                => apply MergeNone
-  | [ |- MergeOption _ _ None]                   => apply MergeNone
-  | [ |- MergeOption None _ (Some ?w)]           => apply MergeRight
-  | [ |- MergeOption _ None (Some ?w)]           => apply MergeLeft
-  | [ |- WF_Circuit _ _ _]                       => econstructor
-  end )); type_check_circ).
+(*
+Definition out (v : Var) (W : WType ) := output (type_var v W).
+*)
 
 (*** Paper Examples ***)
 
-Local Obligation Tactic := type_check_circ.
+(* Local Obligation Tactic := type_check_circ. *)
 
-Program Definition hadamard_measure : Boxed_Circ Qubit Bit :=
-  Box w ⊂ Qubit => 
-    (gate H w w' 
-    (gate meas w' b 
-    (output b))).
+(* I don't like having to specify these at all. 
+   It basically means no more variables. *)
 
-(* Explicit Proof:
+(* Program Definition id_circ : Circuit [Some Qubit] Qubit := output _.
+Next Obligation. type_check_circ. Defined. *)
 
-  unfold hadamard_measure_obligation_1. simpl.
-  econstructor.
-  3: constructor.
-  3: repeat constructor.
-  3: repeat constructor.  
-  repeat constructor.
-  repeat constructor.
-  econstructor.
-  3: constructor.
-  3: repeat constructor.
-  3: repeat constructor.
-  repeat constructor.
-  repeat constructor.
-  constructor.
-  repeat constructor.
-Defined.
+Program Definition id_circ {W} :  Box W W := 
+  box (fun Γ p1 => output p1).
+
+
+(*
+Program Definition id_circ' : Circuit _ _ := 
+  output (type_var q Qubit).
 *)
 
+(*
+Program Definition id_circ : Circuit _ _ := out w Qubit. 
+*)
+
+Check id_circ.
+Print id_circ.
+Eval simpl in id_circ.
+Eval compute in id_circ.
+
+(*
+Eval compute in id_circ'.
+*)
+
+(*
+Program Definition hadamard_c : Circuit [Some Qubit] Qubit :=
+  gate [] H (type_var q Qubit) (fun Γ2 Γ2' M2 p2 => output p2) _ .
+Next Obligation. type_check_circ. Defined.
+Next Obligation. type_check_circ. Defined.
+(*
+Next Obligation. apply merge_r_eq in H1. subst. assumption. Defined.
+Next Obligation. apply MergeNilR. Defined.
+*)
+
+(* Doesn't work. Why not?
+Program Definition hadamard_c : Circuit [Some Qubit] Qubit :=
+  gate [] H (make_pattern q Qubit) (fun _ _ _ _ => output (make_pattern q Qubit)) _ .
+Next Obligation. type_check_circ. Defined.
+Next Obligation. type_check_circ. Defined. *)
+
+Program Definition hadamard_measure_c : Circuit [Some Qubit] Bit :=
+  gate [] H (type_var q Qubit) 
+  (fun Γ2 Γ2' M2 p2 => gate [] meas p2
+  (fun Γ3 Γ3' M3 p3 => output p3) _) _ .
+Next Obligation. type_check_circ. Defined.
+
+Check box.
+*)
+
+Program Definition hadamard_measure : Box Qubit Bit :=
+  box (fun Γ p1 => 
+   gate [] _ H p1 
+  (fun Γ2 Γ2' M2 p2 => gate [] _ meas p2
+  (fun Γ3 Γ3' M3 p3 => output p3))).
+Next Obligation. type_check_circ. Defined.
+Next Obligation. type_check_circ. Defined.
+  
 (* This - correctly - fails to type check!*)
 (*
 Program Definition absurd_circ : Boxed_Circ Qubit (Bit ⊗ Qubit) := 
@@ -137,6 +286,7 @@ Program Definition absurd_circ : Boxed_Circ Qubit (Bit ⊗ Qubit) :=
 Obligation 2. Abort. 
 *)
 
+(*
 Program Definition inSeq {W1 W2 W3 : WType} 
   (c1 : Boxed_Circ W1 W2) (c2 : Boxed_Circ W2 W3) : Boxed_Circ W1 W3  := 
   Box w1 ⊂ W1 =>
@@ -149,12 +299,54 @@ Program Definition inPar {W1 W2 W1' W2'}
     (compose w2 (unbox c w1) (
        compose w2 (unbox c' w1') (output (w2,w2')))).
 Obligation 2. type_check_circ. Admitted. (* subst not yet defined *)
+*)
 
+Program Definition init : Box One Qubit :=
+  if b then (box (fun Γ p1 => gate [] _ init1 p1 (fun Γ2 Γ2' M2 p2 => output p2)))
+       else (box (fun Γ p1 => gate [] _ init0 p1 (fun Γ2 Γ2' M2 p2 => output p2))).
+Next Obligation. type_check_circ. Defined.
+Next Obligation. type_check_circ. Defined.
+Next Obligation. type_check_circ. Defined.
+Next Obligation. type_check_circ. Defined.
 
+(*
 Program Definition init (b : bool) : Boxed_Circ One Qubit := 
   if b then (Box unit ⊂ One => (gate init1 unit w (output w)))
        else (Box unit ⊂ One => (gate init0 unit w (output w))).
+*)
 
+Parameter Δ1 Δ2 Δ3 Δ4 Δ5 : Ctx.
+
+Program Definition bell00 : Box One (Qubit ⊗ Qubit) :=
+(* I don't like this. Would be much simpler if I could force Γ = [] *)
+  box (fun Γ p1 => 
+  (gate [] _ init0 p1
+  (fun Γ2 Γ2' M2 p2 => gate Γ2 _ init0 (())
+  (fun Γ3 Γ3' M3 p3 => gate Γ3 _ (* Γ2'? *) H p2
+  (fun Γ4 Γ4' M4 p4 => gate [] _ CNOT (p3,p4) 
+  (fun Γ5 Γ5' M5 p5 => output p5)))))).
+Next Obligation. type_check_circ. Defined.
+Next Obligation. type_check_circ. Defined.
+Next Obligation. type_check_circ. Defined.
+Next Obligation. type_check_circ. Defined.
+Next Obligation. type_check_circ. Defined.
+Next Obligation. type_check_circ. Defined.
+
+(*
+Program Definition bell00' : Box One (Qubit ⊗ Qubit) :=
+(* I don't like this. Would be much simpler if I could force Γ = [] *)
+  box (fun Γ p1 => 
+  (gate Γ init0 (())
+  (fun Γ2 Γ2' M2 p2 => gate (merge Γ2 Γ) init0 (())
+  (fun Γ3 Γ3' M3 p3 => gate (merge Γ3 Γ) (* Γ2'? *) H p2
+  (fun Γ4 Γ4' M4 p4 => gate Δ4 CNOT (p3,p4) 
+  (fun Γ5 Γ5' M5 p5 => output p5) _ ) _) _) _)).
+Obligation 7. type_check_circ. Defined.
+Obligation 6. erewrite merge_eq. constructor. assumption. Defined.
+Obligation 5. type_check_circ.
+*)  
+
+(*
 Program Definition bell00 : Boxed_Circ One (Qubit ⊗ Qubit) :=
   Box unit ⊂ One =>
     (gate init0 unit a
@@ -162,7 +354,28 @@ Program Definition bell00 : Boxed_Circ One (Qubit ⊗ Qubit) :=
     (gate H a a
     (gate CNot (a,b) (a,b)
     (output (a,b)))))).
+*)
 
+(* Work in progress *)
+Notation "⟨ p1 , p2 , Γ1 , Γ2 ⟩ ↩ p $ exp" := match wproj p with 
+  Datatypes.pair (existT _ Γ1 p1) (existT _ Γ2 p2) => exp end (at level 20).
+
+Program Definition alice : Box (Qubit⊗Qubit) (Bit⊗Bit) :=
+  box (fun Γ qa => 
+  (gate [] _ CNOT qa
+  (fun Γ2 Γ2' M2 p2 => match wproj p2 with Datatypes.pair (existT _ Γq q) (existT _ Γa a) =>
+  (*  let ((existT _ Γ1'' q), (existT _ Γ2'' a)) := wproj p2 in *)
+     gate Γa _ H q
+  (fun Γ3 Γ3' M3 p3 => gate Γa _ meas p3
+  (fun Γ4 Γ4' M4 p4 => gate Γ4 _ meas a 
+  (fun Γ5 Γ5' M5 p5 => output (p4,p5)))) 
+end))).
+Next Obligation. type_check_circ. Defined.
+Next Obligation. type_check_circ. Defined.
+Next Obligation. type_check_circ. Defined.
+Next Obligation. type_check_circ. Defined.
+
+(*
 Program Definition alice : Boxed_Circ (Qubit⊗Qubit) (Bit⊗Bit) :=
   Box (q,a) ⊂ Qubit⊗Qubit =>
     (gate CNot (q,a) (q,a)
@@ -170,6 +383,114 @@ Program Definition alice : Boxed_Circ (Qubit⊗Qubit) (Bit⊗Bit) :=
     (gate meas q x
     (gate meas a y
     (output (x,y)))))).
+*)
+
+(* Have to rename to avoid conflicts *)
+Lemma merge_trans_l : forall Γ1 Γ2 Γ3 Γ4 Γ',
+  MergeCtx Γ1 Γ3 Γ' -> 
+  MergeCtx Γ2 Γ' Γ4 ->
+  MergeCtx (merge Γ1 Γ2) Γ3 Γ4.
+Proof.
+  intros Γ1 Γ2 Γ3 Γ4 Γ' H0 H1.
+  generalize dependent Γ'.
+  generalize dependent Γ4.
+  generalize dependent Γ3.
+  generalize dependent Γ1.
+  induction Γ2.
+  + intros Γ1 Γ3 Γ4 Γ' H0 H1. 
+    apply merge_l_eq in H1.
+    subst.
+    destruct Γ1; assumption.
+  + intros Γ1 Γ3 Γ4 Γ' H0 H1.
+    destruct Γ1.     
+    - simpl. 
+      apply merge_l_eq in H0; subst.
+      assumption.
+    - simpl. 
+      inversion H0; subst.
+      * inversion H1; subst.
+        apply mergeSymm in H1.
+        apply merge_eq in H1.
+        simpl in H1. rewrite H1.
+        constructor.
+      * inversion H1; subst.
+        destruct o, a0, o2, o4; inversion H4; subst; inversion H9; subst; simpl in *;
+        constructor; try constructor; eapply IHΓ2; try apply H7; try apply H10.
+Qed.
+
+Lemma merge_trans_r : forall Γ1 Γ2 Γ3 Γ4 Γ',
+  MergeCtx Γ1 Γ2 Γ' -> 
+  MergeCtx Γ3 Γ' Γ4 ->
+  MergeCtx Γ1 (merge Γ2 Γ3) Γ4.
+Proof.
+  intros Γ1 Γ2 Γ3 Γ4 Γ' H0 H1.
+  apply mergeSymm.
+  eapply merge_trans_l.
+  apply (mergeSymm H0).
+  apply H1.
+Qed.  
+
+Lemma manual_merge_symm : forall Γ1 Γ2, merge Γ1 Γ2 = merge Γ2 Γ1.
+Proof.
+  intros Γ1. 
+  induction Γ1; intros Γ2.
+  destruct Γ2; reflexivity.  
+  destruct Γ2; trivial.
+  simpl. 
+  rewrite IHΓ1.
+  destruct a0, o; reflexivity.
+Qed.
+
+Program Definition bob : Box (Bit⊗Bit⊗Qubit) Qubit :=
+  box (fun Γxyb xyb =>
+    match wproj xyb with Datatypes.pair (existT _ Γx x) (existT _ Γyb yb) =>
+    gate Δ1 _ (bit_control σx) yb 
+     (fun Γyb Γyb' Myb yb =>
+      match wproj yb with Datatypes.pair (existT _ Γy y) (existT _ Γb b) =>
+      gate Δ2 _ (bit_control σz) (x,b)
+       (fun Γxb Γxb' Mxb xb =>
+        match wproj xb with Datatypes.pair (existT _ Γx x) (existT _ Γb b) =>
+        gate Δ3 _ discard y 
+         (fun Γz1 Γz1 Mz1 z1 =>
+          gate Δ4 _ discard x
+          (fun Γz2 Γz2' Mz2 z2 => output b))
+        end)
+      end)
+    end).
+
+
+
+
+Program Definition bob : Box (Bit⊗Bit⊗Qubit) Qubit :=
+  box (fun Γxyb xyb =>
+    match wproj xyb with Datatypes.pair (existT _ Γx x) (existT _ Γyb yb) =>
+    gate Γx _ (bit_control σx) yb 
+     (fun Γyb Γyb' Myb yb =>
+      match wproj yb with Datatypes.pair (existT _ Γy y) (existT _ Γb b) =>
+      gate (merge Γx Γy) _ (bit_control σz) (x,b)
+       (fun Γ2 Γ2' M2 p2 =>
+        match wproj p2 with Datatypes.pair (existT _ Γx x) (existT _ Γb b) =>
+        gate Δ3 _ discard y 
+         (fun Γ3 Γ3' M3 p3 =>
+          gate Δ4 _ discard x
+          (fun Γ4 Γ4' M4 p4 => output b))
+        end)
+      end)
+    end).
+Next Obligation. type_check_circ. Defined.
+Next Obligation. unfold bob_obligation_2. 
+                 apply wproj_merge in Heq_anonymous.
+                 apply wproj_merge in Heq_anonymous0.
+                 clear - Heq_anonymous Heq_anonymous0 Myb.
+                 rewrite manual_merge_symm.
+                 eapply merge_trans_r.
+                 apply (mergeSymm Heq_anonymous).
+                 apply (mergeSymm Myb). Defined.                 
+Next Obligation. type_check_circ.
+                 clear - Heq_anonymous Heq_anonymous0 Myb.
+                 
+
+
 
 Program Definition bob : Boxed_Circ (Bit⊗Bit⊗Qubit) Qubit :=
   Box (x,y,b) ⊂ (Bit⊗Bit⊗Qubit) =>
@@ -190,6 +511,8 @@ Obligation 2. type_check_circ. Admitted.
 
 Parameter run : Circuit -> bool.
 
+Parameter run2 : Boxed_Circ One Bit -> bool.
+
 Program Definition flip : bool := 
   run 
   (gate init0 unit q
@@ -197,6 +520,14 @@ Program Definition flip : bool :=
   (gate meas q b
   (output b)))).
 
+
+Program Definition flip2 : bool := 
+  run2 
+  (Box unit ⊂ One => 
+  (gate init0 unit q
+  (gate H q q
+  (gate meas q b
+  (output b))))).
 
 
 (* *)
